WIP

src/Init/Data/String/Lemmas/g.lean
@@ -7,15 +7,21 @@ module
 
 prelude
 public import Init.Data.String.Slice
+import all Init.Data.String.Slice
+import all Init.Data.String.Pattern.Basic
 import all Init.Data.String.Pattern.Pred
 import all Init.Data.String.Positions
 import Init.Data.Iterators.Lemmas.Basic
 import Init.Data.Iterators.Lemmas.Consumers.Collect
 import Init.Data.Iterators.Lemmas.Combinators.FilterMap
+import Init.Data.String.Lemmas.Order
+import Init.Data.String.Lemmas.Basic
+import Init.Data.String.Grind
+import Init.Grind
 
 namespace List
 
--- From Batteries
+section FromBatteries
 
 /--
 Split a list at every element satisfying a predicate. The separators are not in the result.
@@ -30,6 +36,31 @@ def splitOnP (P : α → Bool) (l : List α) : List (List α) := go l [] where
   | [], acc => [acc.reverse]
   | a :: t, acc => if P a then acc.reverse :: go t [] else go t (a::acc)
 
+/-- `IsChain R l` means that `R` holds between adjacent elements of `l`.
+```
+IsChain R [a, b, c, d] ↔ R a b ∧ R b c ∧ R c d
+``` -/
+inductive IsChain (R : α → α → Prop) : List α → Prop where
+  /-- A list of length 0 is a chain. -/
+  | nil : IsChain R []
+  /-- A list of length 1 is a chain. -/
+  | singleton (a : α) : IsChain R [a]
+  /-- If `a` relates to `b` and `b::l` is a chain, then `a :: b :: l` is also a chain. -/
+  | cons_cons (hr : R a b) (h : IsChain R (b :: l)) : IsChain R (a :: b :: l)
+
+end FromBatteries
+
+section FromMathlib
+
+theorem isChain_map_of_isChain {S : β → β → Prop} (f : α → β) (H : ∀ a b : α, R a b → S (f a) (f b))
+    {l : List α} (p : IsChain R l) : IsChain S (map f l) := sorry
+
+end FromMathlib
+
+def last : (l : List α) → (hl : l ≠ []) → α
+  | a :: [], h => a
+  | a :: b :: bs, h => (b :: bs).last (by simp)
+
 end List
 
 namespace String.Slice
@@ -41,7 +72,7 @@ theorem PosIterator.step_eq_if
     else
       .yield ⟨⟨i.internalState.currPos.next h⟩⟩ ⟨i.internalState.currPos, h⟩ := by
   simp [Std.Iter.step, Std.IterM.step, Std.Iterator.step]
-  split <;> simp
+  split <;> simp [Std.IterM.toIter_mk']
 
 theorem PosIterator.toList_endPos {s : Slice} :
     (Std.Iter.mk (PosIterator.mk s.endPos)).toList = [] := by
@@ -57,10 +88,81 @@ theorem PosIterator.toList_eq_cons {s : Slice}
 
 namespace Pattern
 
-class LawfulForwardPattern {ρ : Type} (pat : ρ) [ForwardPattern pat] : Prop where
-  isSome_dropPrefix? (s : Slice) : (s.dropPrefix? pat).isSome = s.startsWith pat
+namespace SearchStep
 
--- instance
+def startPos {s : Slice} (st : SearchStep s) : s.Pos :=
+  match st with
+  | .rejected startPos _ => startPos
+  | .matched startPos _ => startPos
+
+@[simp]
+theorem startPos_rejected {s : Slice} {p q : s.Pos} : (SearchStep.rejected p q).startPos = p := rfl
+
+@[simp]
+theorem startPos_matched {s : Slice} {p q : s.Pos} : (SearchStep.matched p q).startPos = p := rfl
+
+def endPos {s : Slice} (st : SearchStep s) : s.Pos :=
+  match st with
+  | .rejected _ endPos => endPos
+  | .matched _ endPos => endPos
+
+@[simp]
+theorem endPos_rejected {s : Slice} {p q : s.Pos} : (SearchStep.rejected p q).endPos = q := rfl
+
+@[simp]
+theorem endPos_matched {s : Slice} {p q : s.Pos} : (SearchStep.matched p q).endPos = q := rfl
+
+end SearchStep
+
+structure IsMatchList (s : Slice) (l : List (SearchStep s)) : Prop where
+  exists_le_and_lt : ∀ p : s.Pos, p ≠ s.endPos → ∃ st ∈ l, st.startPos ≤ p ∧ p < st.endPos
+  lt : ∀ st ∈ l, st.startPos < st.endPos
+  isChain : l.IsChain (fun l r => l.endPos = r.startPos)
+
+class LawfulToForwardSearcher {ρ : Type} {σ : Slice → Type} (pat : ρ) [ToForwardSearcher pat σ]
+    [∀ s, Std.Iterator (σ s) Id (SearchStep s)] [∀ s, Std.Iterators.Finite (σ s) Id] where
+  isMatchList (s : Slice) : IsMatchList s (ToForwardSearcher.toSearcher pat s).toList
+
+class LawfulForwardPattern {ρ : Type} (pat : ρ) [ForwardPattern pat] : Prop where
+  isSome_dropPrefix? (s : Slice) : (ForwardPattern.dropPrefix? pat s).isSome = ForwardPattern.startsWith pat s
+  dropPrefix?_ne_startPos (s : Slice) (p : s.Pos) : ForwardPattern.dropPrefix? pat s = some p → p ≠ s.startPos
+
+theorem ForwardPattern.startsWith_defaultImplementation {ρ : Type} {σ : Slice → Type}
+    [∀ s, Std.Iterator (σ s) Id (SearchStep s)] {pat : ρ} [ToForwardSearcher pat σ]
+    [∀ s, Std.IteratorLoop (σ s) Id Id] (s : Slice) :
+    letI := ForwardPattern.defaultImplementation (pat := pat)
+    ForwardPattern.startsWith pat s = ForwardPattern.defaultStartsWith pat s := rfl
+
+theorem ForwardPattern.dropPrefix?_defaultImplementation {ρ : Type} {σ : Slice → Type}
+    [∀ s, Std.Iterator (σ s) Id (SearchStep s)] {pat : ρ} [ToForwardSearcher pat σ]
+    [∀ s, Std.IteratorLoop (σ s) Id Id] (s : Slice) :
+    letI := ForwardPattern.defaultImplementation (pat := pat)
+    ForwardPattern.dropPrefix? pat s = ForwardPattern.defaultDropPrefix? pat s := rfl
+
+theorem LawfulForwardPattern.defaultImplementation {ρ : Type} {σ : Slice → Type}
+    [∀ s, Std.Iterator (σ s) Id (SearchStep s)] {pat : ρ} [ToForwardSearcher pat σ]
+    [∀ s, Std.Iterators.Finite (σ s) Id] [LawfulToForwardSearcher pat]
+    [∀ s, Std.IteratorLoop (σ s) Id Id] :
+    letI : ForwardPattern pat := ForwardPattern.defaultImplementation (pat := pat)
+    LawfulForwardPattern pat := by
+  letI : ForwardPattern pat := ForwardPattern.defaultImplementation (pat := pat)
+  refine ⟨fun s => ?_, fun s p => ?_⟩
+  · rw [ForwardPattern.dropPrefix?_defaultImplementation,
+      ForwardPattern.startsWith_defaultImplementation,
+      ForwardPattern.defaultStartsWith, ForwardPattern.defaultDropPrefix?]
+    split <;> simp
+  · simp
+    rw [ForwardPattern.dropPrefix?_defaultImplementation, ForwardPattern.defaultDropPrefix?]
+    
+
+    sorry
+
+instance {pat : Char → Bool} : LawfulForwardPattern pat := .defaultImplementation
+
+-- def stupidSplit {ρ : Type} [ForwardPattern pat] (pat : ρ) (s : Slice) : List (SearchStep s) :=
+--   go s.startPos
+-- where
+--   go (pos : s.Pos)
 
 theorem ForwardCharPredSearcher.step_eq_if
     {i : Std.Iter (α := ForwardCharPredSearcher p s) (SearchStep s)} :
@@ -77,8 +179,8 @@ theorem ForwardCharPredSearcher.step_eq_if
   split
   · simp
   · split
-    · simp
-    · simp
+    · simp [Std.IterM.toIter_mk']
+    · simp [Std.IterM.toIter_mk']
 
 theorem bar {p : Char → Bool} {s : Slice} {pos : s.Pos} :
     (Std.Iter.mk (ForwardCharPredSearcher.mk (p := p) pos)).toList =
@@ -111,6 +213,92 @@ theorem ForwardCharPredSearcher.toList_iter {p : Char → Bool} {s : Slice} :
         else
           .rejected pos.1 (pos.1.next pos.2))) := by
   rw [ForwardCharPredSearcher.iter, bar, Slice.positions]
+
+theorem ForwardCharPredSearcher.toList_toSearcher {p : Char → Bool} {s : Slice} :
+    (ToForwardSearcher.toSearcher p s).toList =
+      (s.positions.toList.map (fun pos =>
+        if p (pos.1.get pos.2) then
+          .matched pos.1 (pos.1.next pos.2)
+        else
+          .rejected pos.1 (pos.1.next pos.2))) :=
+  toList_iter
+
+def positionsFrom {s : Slice} (p : s.Pos) : List { pos // pos ≠ s.endPos } :=
+  if h : p = s.endPos then [] else ⟨p, h⟩ :: positionsFrom (p.next h)
+termination_by p
+
+@[simp]
+theorem positionsFrom_endPos {s : Slice} : positionsFrom s.endPos = [] := by
+  simp [positionsFrom]
+
+theorem positionsFrom_eq_cons {s : Slice} {p : s.Pos} (h : p ≠ s.endPos) :
+    positionsFrom p = ⟨p, h⟩ :: positionsFrom (p.next h) := by
+  rw [positionsFrom]
+  simp [h]
+
+theorem mem_positionsFrom {s : Slice} {p q : s.Pos} (h : q ≠ s.endPos) :
+    ⟨q, h⟩ ∈ positionsFrom p ↔ p ≤ q := by
+  induction p using WellFounded.induction Slice.Pos.wellFounded_gt with | h p ih
+  by_cases h' : p = s.endPos
+  · simp [*]
+  · rw [positionsFrom_eq_cons h']
+    simp only [ne_eq, List.mem_cons, Subtype.mk.injEq, ih (p.next h') (by simp)]
+    rw [Slice.Pos.next_le_iff_lt]
+    grind
+
+theorem PosIterator.step_eq_if {s : Slice} (p : s.Pos) :
+    (Std.Iter.mk (PosIterator.mk p)).step.val =
+      if h : p = s.endPos then
+        .done
+      else
+        .yield ⟨⟨p.next h⟩⟩ ⟨p, h⟩ := by
+  simp [Std.Iter.step, Std.IterM.step, Std.Iterator.step]
+  split
+  · simp
+  · simp [Std.IterM.toIter_mk']
+
+theorem PosIterator.toList_eq {s : Slice} (p : s.Pos) :
+    (Std.Iter.mk (PosIterator.mk p)).toList = positionsFrom p := by
+  induction p using WellFounded.induction Slice.Pos.wellFounded_gt with | h pos ih
+  rw [Std.Iter.toList_eq_match_step, PosIterator.step_eq_if]
+  by_cases h : pos = s.endPos
+  · simp [h]
+  · simp [h]
+    rw [ih _ (by simp), positionsFrom_eq_cons h]
+
+theorem toList_positions {s : Slice} : s.positions.toList = positionsFrom s.startPos := by
+  rw [positions, PosIterator.toList_eq]
+
+theorem isChain_positionsFrom {s : Slice} {p : s.Pos} :
+    List.IsChain (fun p q => q.1 = p.1.next p.2) (positionsFrom p) := by
+  induction p using WellFounded.induction Slice.Pos.wellFounded_gt with | h p ih
+  by_cases h : p = s.endPos
+  · simp [h, List.IsChain.nil]
+  · rw [positionsFrom_eq_cons h]
+    by_cases h' : p.next h = s.endPos
+    · simp [h', List.IsChain.singleton]
+    · rw [positionsFrom_eq_cons h']
+      apply List.IsChain.cons_cons (by simp)
+      rw [← positionsFrom_eq_cons]
+      apply ih _ (by simp)
+
+instance {p : Char → Bool} : LawfulToForwardSearcher p where
+  isMatchList s := by
+    rw [ForwardCharPredSearcher.toList_toSearcher]
+    simp [toList_positions]
+    refine ⟨?_, fun st => ?_, ?_⟩
+    · intro q hq
+      simp only [List.mem_map, Subtype.exists, mem_positionsFrom, Pos.startPos_le, true_and]
+      refine ⟨if p (q.get hq) then SearchStep.matched q (q.next hq)
+        else SearchStep.rejected q (q.next hq), ⟨q, hq, by simp⟩, ?_⟩
+      split <;> simp
+    · simp [mem_positionsFrom]
+      intro p hp
+      split <;> rintro rfl <;> simp
+    · apply List.isChain_map_of_isChain _ _ isChain_positionsFrom
+      rintro ⟨a, ha⟩ ⟨b, hb⟩ rfl
+      simp only
+      split <;> split <;> simp
 
 end Pattern
 
