src/Init/Data/Iterators/Basic.lean
@@ -401,7 +401,6 @@ theorem internalState_toIterM {α m β} (it : α) :
 theorem Iter.internalState_toIterM {α β} (it : Std.Iter (α := α) β) :
     it.toIterM.internalState = it.internalState := rfl
 
-@[simp]
 theorem IterM.toIter_mk' {α β} (it : α) :
     (Std.IterM.mk' (β := β) it).toIter = ⟨it⟩ := rfl
 
