src/Init/Data/String/Lemmas/Order.lean
@@ -1,0 +1,42 @@
+/-
+Copyright (c) 2026 Lean FRO, LLC. All rights reserved.
+Released under Apache 2.0 license as described in the file LICENSE.
+Author: Markus Himmel
+-/
+module
+
+prelude
+public import Init.Data.String.Basic
+import Init.Data.String.Grind
+import Init.Data.String.Lemmas.Basic
+
+public section
+
+namespace String
+
+@[simp]
+theorem Slice.Pos.next_le_iff_lt {s : Slice} {p q : s.Pos} {h} : p.next h ≤ q ↔ p < q :=
+  ⟨fun h => Std.lt_of_lt_of_le lt_next h, next_le_of_lt⟩
+
+@[simp]
+theorem Pos.next_le_iff_lt {s : String} {p q : s.Pos} {h} : p.next h ≤ q ↔ p < q := by
+  rw [next, Pos.ofToSlice_le_iff, ← Pos.toSlice_lt_toSlice_iff]
+  exact Slice.Pos.next_le_iff_lt
+
+@[simp]
+theorem Slice.Pos.le_startPos {s : Slice} (p : s.Pos) : p ≤ s.startPos ↔ p = s.startPos :=
+  ⟨fun h => Std.le_antisymm h (startPos_le _), by simp +contextual⟩
+
+@[simp]
+theorem Slice.Pos.endPos_le {s : Slice} (p : s.Pos) : s.endPos ≤ p ↔ p = s.endPos :=
+  ⟨fun h => Std.le_antisymm (le_endPos _) h, by simp +contextual⟩
+
+@[simp]
+theorem Pos.le_startPos {s : String} (p : s.Pos) : p ≤ s.startPos ↔ p = s.startPos :=
+  ⟨fun h => Std.le_antisymm h (startPos_le _), by simp +contextual⟩
+
+@[simp]
+theorem Pos.endPos_le {s : String} (p : s.Pos) : s.endPos ≤ p ↔ p = s.endPos :=
+  ⟨fun h => Std.le_antisymm (le_endPos _) h, by simp +contextual⟩
+
+end String
